<?xml version="1.0" encoding="utf-8"?>
<rdf:RDF
  xmlns:dct="http://purl.org/dc/terms/"
  xmlns:owl="http://www.w3.org/2002/07/owl#"
  xmlns:rdfs="http://www.w3.org/2000/01/rdf-schema#"
  xmlns:rdf="http://www.w3.org/1999/02/22-rdf-syntax-ns#"
  xmlns:skos="http://www.w3.org/2004/02/skos/core#"
>
  <owl:DatatypeProperty rdf:about="http://e-editiones.ch/ontology/organization#hasNameLiteral">
    <rdfs:label xml:lang="de">Personenorganisation hat Namenliteral</rdfs:label>
    <rdfs:label xml:lang="en">person organization has name literal</rdfs:label>
    <rdfs:comment xml:lang="en">Relating a person organization to the literal of a name of that organization.</rdfs:comment>
    <rdfs:subPropertyOf rdf:resource="http://e-editiones.ch/ontology/text#hasNameLiteral"/>
    <rdfs:isDefinedBy rdf:resource="http://e-editiones.ch/ontology/organization#"/>
    <rdfs:range rdf:resource="http://www.w3.org/2000/01/rdf-schema#Literal"/>
    <rdfs:domain rdf:resource="http://e-editiones.ch/ontology/organization#Organization"/>
  </owl:DatatypeProperty>
  <rdfs:Class rdf:about="http://e-editiones.ch/ontology/organization#Library">
    <rdfs:comment xml:lang="en">Organization having a role of preserving and making accessible information carriers to a defined community for reference or borrowing. An information carrier can be a book, periodical, newspaper, manuscript, film, map, print, also in microform, CD, cassette, videotape, DVD, Blu-ray Disc, e-book, audiobook, database, and other document format.</rdfs:comment>
    <rdfs:subClassOf rdf:resource="http://e-editiones.ch/ontology/organization#CulturalHeritageInstitution"/>
    <rdfs:label xml:lang="fr">bibliothèque</rdfs:label>
    <rdfs:label xml:lang="it">biblioteca</rdfs:label>
    <rdfs:label xml:lang="en">library</rdfs:label>
    <rdfs:isDefinedBy rdf:resource="http://e-editiones.ch/ontology/organization#"/>
    <rdfs:label xml:lang="de">Bibliothek</rdfs:label>
  </rdfs:Class>
  <owl:ObjectProperty rdf:about="http://e-editiones.ch/ontology/organization#isMemberOfReligiousOrganization">
    <rdfs:label xml:lang="en">is member of religious organization</rdfs:label>
    <rdfs:isDefinedBy rdf:resource="http://e-editiones.ch/ontology/organization#"/>
    <rdfs:subPropertyOf>
      <owl:ObjectProperty rdf:about="http://e-editiones.ch/ontology/organization#isMemberOf">
        <rdfs:comment xml:lang="en">Relating a person to an organization the person is a member of.</rdfs:comment>
        <rdfs:isDefinedBy rdf:resource="http://e-editiones.ch/ontology/organization#"/>
        <rdfs:label xml:lang="de">ist Mitglied einer Personenorganisation</rdfs:label>
        <rdfs:range rdf:resource="http://e-editiones.ch/ontology/organization#Organization"/>
        <rdfs:domain rdf:resource="http://e-editiones.ch/ontology/human#Person"/>
        <rdfs:label xml:lang="en">is member of person organization</rdfs:label>
        <rdfs:subPropertyOf rdf:resource="http://e-editiones.ch/ontology/human#isMemberOf"/>
      </owl:ObjectProperty>
    </rdfs:subPropertyOf>
    <rdfs:label xml:lang="de">ist Mitglied einer religiösen Organisation</rdfs:label>
    <rdfs:domain rdf:resource="http://e-editiones.ch/ontology/organization#ReligiousPerson"/>
    <rdfs:range rdf:resource="http://e-editiones.ch/ontology/organization#ReligiousOrganization"/>
    <rdfs:comment xml:lang="en">Relating a person to a religious organization the person is a member of.</rdfs:comment>
  </owl:ObjectProperty>
  <owl:ObjectProperty rdf:about="http://e-editiones.ch/ontology/organization#isMemberOfAdministration">
    <rdfs:comment xml:lang="en">Relating a person to an administration organization the person is a member of.</rdfs:comment>
    <rdfs:subPropertyOf rdf:resource="http://e-editiones.ch/ontology/organization#isMemberOf"/>
    <rdfs:range>
      <rdf:Description rdf:nodeID="ub39bL196C13">
        <rdfs:subClassOf>
          <owl:Restriction rdf:nodeID="ub39bL196C57">
            <owl:onProperty rdf:resource="http://e-editiones.ch/ontology/organization#hasRole"/>
            <owl:someValuesFrom rdf:resource="http://e-editiones.ch/ontology/organization#Administration"/>
          </owl:Restriction>
        </rdfs:subClassOf>
        <rdfs:subClassOf rdf:resource="http://e-editiones.ch/ontology/organization#Organization"/>
      </rdf:Description>
    </rdfs:range>
    <rdfs:label xml:lang="en">is member of administration</rdfs:label>
    <rdfs:isDefinedBy rdf:resource="http://e-editiones.ch/ontology/organization#"/>
    <rdfs:label xml:lang="de">ist Mitglied einer Verwaltung</rdfs:label>
    <rdfs:domain rdf:resource="http://e-editiones.ch/ontology/human#Person"/>
  </owl:ObjectProperty>
  <owl:ObjectProperty rdf:about="http://e-editiones.ch/ontology/organization#actsIn">
    <rdfs:subPropertyOf rdf:resource="http://e-editiones.ch/ontology/human#actsIn"/>
    <rdfs:domain rdf:resource="http://e-editiones.ch/ontology/organization#Organization"/>
    <rdfs:label xml:lang="en">person organization acts in</rdfs:label>
    <rdfs:isDefinedBy rdf:resource="http://e-editiones.ch/ontology/organization#"/>
    <rdfs:comment xml:lang="en">Relating a person organization to an action it acts in.</rdfs:comment>
    <rdfs:label xml:lang="de">Personenorganisation agiert in</rdfs:label>
    <rdfs:range rdf:resource="http://e-editiones.ch/ontology/human#Action"/>
  </owl:ObjectProperty>
  <rdfs:Class rdf:about="http://e-editiones.ch/ontology/organization#PoliticalOrganization">
    <rdfs:isDefinedBy rdf:resource="http://e-editiones.ch/ontology/organization#"/>
    <rdfs:label xml:lang="en">political organization</rdfs:label>
    <rdfs:comment xml:lang="en">Organization being involved in politics.</rdfs:comment>
    <rdfs:label xml:lang="de">politische Organisation</rdfs:label>
    <rdfs:subClassOf rdf:resource="http://e-editiones.ch/ontology/organization#Organization"/>
  </rdfs:Class>
  <rdfs:Class rdf:about="http://e-editiones.ch/ontology/organization#Politician">
    <rdfs:label xml:lang="de">Politikerrolle einer Person</rdfs:label>
    <rdfs:isDefinedBy rdf:resource="http://e-editiones.ch/ontology/organization#"/>
    <rdfs:subClassOf rdf:resource="http://e-editiones.ch/ontology/human#OccupationalRole"/>
    <rdfs:label xml:lang="en">politician role of person</rdfs:label>
    <rdfs:comment xml:lang="en">Occupational role of being professionally involved in politics, especially as a holder of an elected office.</rdfs:comment>
  </rdfs:Class>
  <owl:ObjectProperty rdf:about="http://e-editiones.ch/ontology/organization#isMemberOfCompany">
    <rdfs:range rdf:resource="http://e-editiones.ch/ontology/organization#Company"/>
    <rdfs:label xml:lang="de">ist Mitglied einer Firma</rdfs:label>
    <rdfs:domain rdf:resource="http://e-editiones.ch/ontology/human#Person"/>
    <rdfs:label xml:lang="en">is member of company</rdfs:label>
    <rdfs:isDefinedBy rdf:resource="http://e-editiones.ch/ontology/organization#"/>
    <rdfs:comment xml:lang="en">Relating a person to a company the person is a member of.</rdfs:comment>
    <rdfs:subPropertyOf rdf:resource="http://e-editiones.ch/ontology/organization#isMemberOf"/>
  </owl:ObjectProperty>
  <owl:Ontology rdf:about="http://e-editiones.ch/ontology/organization">
    <dct:license rdf:resource="http://creativecommons.org/licenses/by/3.0/"/>
    <dct:title xml:lang="en">An ontology about person organization</dct:title>
    <dct:description xml:lang="en">Formal description of organization involving persons, general subclasses, related classes and properties.</dct:description>
    <dct:contributor xml:lang="en">Rebekka Plüss, research assistant and software developer, University of Basel, Switzerland</dct:contributor>
    <owl:versionInfo rdf:datatype="http://www.w3.org/2001/XMLSchema#date">2020-06-11</owl:versionInfo>
    <dct:publisher xml:lang="en">Universities of Basel, Bern, and Zürich, Switzerland</dct:publisher>
    <dct:creator xml:lang="en">Hans Cools, MD, knowledge engineer, ontologist, software developer, University of Basel, Switzerland</dct:creator>
  </owl:Ontology>
  <rdfs:Class rdf:about="http://e-editiones.ch/ontology/organization#MasonicLodge">
    <rdfs:isDefinedBy rdf:resource="http://e-editiones.ch/ontology/organization#"/>
    <rdfs:label xml:lang="de">Freimaurerloge</rdfs:label>
    <rdfs:label xml:lang="en">Masonic lodge</rdfs:label>
    <rdfs:subClassOf rdf:resource="http://e-editiones.ch/ontology/organization#Organization"/>
    <rdfs:comment xml:lang="en">Organizational unit of Freemasonry.</rdfs:comment>
  </rdfs:Class>
  <rdfs:Class rdf:about="http://e-editiones.ch/ontology/organization#Creator">
    <rdfs:subClassOf rdf:resource="http://e-editiones.ch/ontology/creating#AgentCreator"/>
    <rdfs:label xml:lang="de">Erstellerrolle einer Organisation</rdfs:label>
    <rdfs:comment xml:lang="en">Creator as role of an organization.</rdfs:comment>
    <rdfs:subClassOf rdf:resource="http://e-editiones.ch/ontology/organization#Role"/>
    <rdfs:label xml:lang="en">creator role of organization</rdfs:label>
    <rdfs:isDefinedBy rdf:resource="http://e-editiones.ch/ontology/organization#"/>
  </rdfs:Class>
  <rdfs:Class rdf:about="http://e-editiones.ch/ontology/organization#Archive">
    <rdfs:isDefinedBy rdf:resource="http://e-editiones.ch/ontology/organization#"/>
    <rdfs:subClassOf rdf:resource="http://e-editiones.ch/ontology/organization#CulturalHeritageInstitution"/>
    <rdfs:label xml:lang="it">archivio</rdfs:label>
    <rdfs:comment xml:lang="en">Organization having a role of systematic collection, preservation, care and making accessible files, records and documents on different information carriers. There are state archives which document the activities of the administration of the state, or there are archives that collect documents on specific topics - f.e. Social Archive or Women's Archive.</rdfs:comment>
    <rdfs:label xml:lang="en">archive</rdfs:label>
    <rdfs:label xml:lang="de">Archiv</rdfs:label>
    <rdfs:label xml:lang="fr">archive</rdfs:label>
  </rdfs:Class>
  <rdfs:Class rdf:about="http://e-editiones.ch/ontology/organization#Museum">
    <rdfs:subClassOf rdf:resource="http://e-editiones.ch/ontology/organization#CulturalHeritageInstitution"/>
    <rdfs:label xml:lang="en">museum</rdfs:label>
    <rdfs:label xml:lang="de">Museum</rdfs:label>
    <rdfs:isDefinedBy rdf:resource="http://e-editiones.ch/ontology/organization#"/>
    <rdfs:comment xml:lang="en">Organization having roles of preserving and exhibiting objects of historical, scientific, artistic, or cultural interest in a special building also called museum.</rdfs:comment>
  </rdfs:Class>
  <rdfs:Class rdf:about="http://e-editiones.ch/ontology/organization#CulturalHeritageInstitution">
    <rdfs:label xml:lang="de">Kulturerbeinstitution</rdfs:label>
    <rdfs:comment xml:lang="en">Organization having a role of preserving a repository of public knowledge, such as a library, an archive, museum, sites and monuments record, clearinghouse, a provider of a digital library, and a data aggregation service, which serve as memories for given societies or mankind.</rdfs:comment>
    <rdfs:subClassOf rdf:resource="http://e-editiones.ch/ontology/organization#Organization"/>
    <rdfs:isDefinedBy rdf:resource="http://e-editiones.ch/ontology/organization#"/>
    <rdfs:subClassOf>
      <owl:Restriction rdf:nodeID="ub39bL101C45">
        <owl:someValuesFrom rdf:resource="http://e-editiones.ch/ontology/organization#Preserver"/>
        <owl:onProperty rdf:resource="http://e-editiones.ch/ontology/organization#hasRole"/>
      </owl:Restriction>
    </rdfs:subClassOf>
    <rdfs:label xml:lang="en">cultural heritage institution</rdfs:label>
  </rdfs:Class>
  <rdfs:Class rdf:about="http://e-editiones.ch/ontology/organization#Administration">
    <rdfs:label xml:lang="en">administration</rdfs:label>
    <rdfs:label xml:lang="de">Verwaltung</rdfs:label>
    <rdfs:comment xml:lang="en">Role of an organization administering a group of people on any level, e.g. international, national, regional or city level.</rdfs:comment>
    <rdfs:subClassOf rdf:resource="http://e-editiones.ch/ontology/organization#Role"/>
    <rdfs:isDefinedBy rdf:resource="http://e-editiones.ch/ontology/organization#"/>
  </rdfs:Class>
  <rdfs:Class rdf:about="http://e-editiones.ch/ontology/organization#Company">
    <rdfs:comment xml:lang="en">Organization having primarily an economical role.</rdfs:comment>
    <rdfs:label xml:lang="de">Betrieb</rdfs:label>
    <rdfs:subClassOf rdf:resource="http://e-editiones.ch/ontology/organization#Organization"/>
    <rdfs:isDefinedBy rdf:resource="http://e-editiones.ch/ontology/organization#"/>
    <rdfs:label xml:lang="en">company</rdfs:label>
  </rdfs:Class>
  <rdfs:Class rdf:about="http://e-editiones.ch/ontology/organization#Organization">
    <rdfs:label xml:lang="de">Personenorganisation</rdfs:label>
    <owl:disjointWith rdf:resource="http://e-editiones.ch/ontology/human#Person"/>
    <rdfs:subClassOf rdf:resource="http://e-editiones.ch/ontology/human#Group"/>
    <rdfs:subClassOf rdf:resource="http://iflastandards.info/ns/fr/frbr/frbroo/F11_Corporate_Body"/>
    <rdfs:subClassOf rdf:resource="http://e-editiones.ch/ontology/agent#Organization"/>
    <rdfs:subClassOf rdf:resource="http://xmlns.com/foaf/0.1/Organization"/>
    <skos:note xml:lang="en">An organization can be a legal person.</skos:note>
    <rdfs:label xml:lang="en">person organization</rdfs:label>
    <rdfs:comment xml:lang="en">Organized group of persons.</rdfs:comment>
    <rdfs:isDefinedBy rdf:resource="http://e-editiones.ch/ontology/organization#"/>
  </rdfs:Class>
  <rdfs:Class rdf:about="http://e-editiones.ch/ontology/organization#Role">
    <rdfs:label xml:lang="de">Rolle einer Organisation</rdfs:label>
    <rdfs:subClassOf rdf:resource="http://e-editiones.ch/ontology/human#GroupRole"/>
    <rdfs:comment xml:lang="en">Role of a person organization.</rdfs:comment>
    <rdfs:label xml:lang="en">organization's role</rdfs:label>
    <rdfs:isDefinedBy rdf:resource="http://e-editiones.ch/ontology/organization#"/>
  </rdfs:Class>
  <rdfs:Class rdf:about="http://e-editiones.ch/ontology/organization#ReligiousOrganization">
    <rdfs:label xml:lang="en">religious organization</rdfs:label>
    <rdfs:label xml:lang="de">religiöse Organisation</rdfs:label>
    <rdfs:comment xml:lang="en">Organization of religious persons.</rdfs:comment>
    <rdfs:isDefinedBy rdf:resource="http://e-editiones.ch/ontology/organization#"/>
    <rdfs:subClassOf rdf:resource="http://e-editiones.ch/ontology/organization#Organization"/>
  </rdfs:Class>
  <rdfs:Class rdf:about="http://e-editiones.ch/ontology/organization#ReligiousPerson">
    <rdfs:comment xml:lang="en">Person having religious faith or believing.</rdfs:comment>
    <rdfs:isDefinedBy rdf:resource="http://e-editiones.ch/ontology/organization#"/>
    <rdfs:label xml:lang="de">religiöse Person</rdfs:label>
    <rdfs:label xml:lang="fr">personne réligieuse</rdfs:label>
    <rdfs:label xml:lang="en">religious person</rdfs:label>
    <rdfs:subClassOf rdf:resource="http://e-editiones.ch/ontology/human#Person"/>
  </rdfs:Class>
  <rdfs:Class rdf:about="http://e-editiones.ch/ontology/organization#Preserver">
    <rdfs:subClassOf rdf:resource="http://e-editiones.ch/ontology/organization#Role"/>
    <rdfs:label xml:lang="en">preserver role of organization</rdfs:label>
    <rdfs:isDefinedBy rdf:resource="http://e-editiones.ch/ontology/organization#"/>
    <rdfs:subClassOf rdf:resource="http://e-editiones.ch/ontology/human#AgentPreserver"/>
    <rdfs:comment xml:lang="en">Role of a person organization as preserver.</rdfs:comment>
    <rdfs:label xml:lang="de">Erhalterrolle einer Organisation</rdfs:label>
  </rdfs:Class>
  <owl:ObjectProperty rdf:about="http://e-editiones.ch/ontology/organization#hasRole">
    <rdfs:domain rdf:resource="http://e-editiones.ch/ontology/organization#Organization"/>
    <rdfs:isDefinedBy rdf:resource="http://e-editiones.ch/ontology/organization#"/>
    <rdfs:comment xml:lang="en">Relating a person organization to a role it has.</rdfs:comment>
    <rdfs:label xml:lang="de">Personenorganisation hat Rolle</rdfs:label>
    <rdfs:label xml:lang="en">person organization has role</rdfs:label>
    <rdfs:subPropertyOf rdf:resource="http://e-editiones.ch/ontology/human#groupHasRole"/>
    <rdfs:range rdf:resource="http://e-editiones.ch/ontology/organization#Role"/>
  </owl:ObjectProperty>
</rdf:RDF>
