<?xml version="1.0" encoding="utf-8"?>
<rdf:RDF
  xmlns:dct="http://purl.org/dc/terms/"
  xmlns:rdfs="http://www.w3.org/2000/01/rdf-schema#"
  xmlns:calendar="http://e-editiones.ch/ontology/calendar#"
  xmlns:skos="http://www.w3.org/2004/02/skos/core#"
  xmlns:owl="http://www.w3.org/2002/07/owl#"
  xmlns:rdf="http://www.w3.org/1999/02/22-rdf-syntax-ns#"
>
  <calendar:Calendar rdf:about="http://e-editiones.ch/ontology/calendar#prolepticGregorianCalendar">
    <rdfs:isDefinedBy rdf:resource="http://e-editiones.ch/ontology/calendar#"/>
    <rdfs:label xml:lang="de">proleptischer gregorianischer Kalender</rdfs:label>
    <rdfs:label xml:lang="en">proleptic Gregorian calendar</rdfs:label>
    <rdfs:comment xml:lang="en">Produced by extending the Gregorian calendar backward to dates preceding its introduction on 15 October 1582.</rdfs:comment>
    <rdfs:label xml:lang="fr">calendrier gr√©gorien proleptique</rdfs:label>
    <skos:note xml:lang="en">There is no proleptic Gregorian year 0. Year 1 BC is followed by year 1 AD.</skos:note>
    <rdfs:label xml:lang="it">calendario gregoriano proleptico</rdfs:label>
  </calendar:Calendar>
  <owl:ObjectProperty rdf:about="http://e-editiones.ch/ontology/calendar#dateLiteralToDate">
    <rdfs:label xml:lang="de">Datumliteral zu Datum</rdfs:label>
    <rdfs:comment xml:lang="en">Relating a calendar date as a literal list to the list with a calendar-dependent date typed literal.</rdfs:comment>
    <skos:note xml:lang="en">Used in the premise of an N3-rule to invoke the backward N3-rule converting a date literal list to the list with the calendar-dependent date typed literal and the Julian Day Number for temporal reasoning.</skos:note>
    <rdfs:range rdf:resource="http://www.w3.org/1999/02/22-rdf-syntax-ns#List"/>
    <rdfs:domain rdf:resource="http://www.w3.org/1999/02/22-rdf-syntax-ns#List"/>
    <rdfs:label xml:lang="en">date literal to date</rdfs:label>
    <rdfs:isDefinedBy rdf:resource="http://e-editiones.ch/ontology/calendar#"/>
  </owl:ObjectProperty>
  <owl:ObjectProperty rdf:about="http://e-editiones.ch/ontology/calendar#hasCalendar">
    <rdfs:comment xml:lang="en">Relating an event to a calendar.</rdfs:comment>
    <rdfs:range rdf:resource="http://e-editiones.ch/ontology/calendar#Calendar"/>
    <rdfs:label xml:lang="en">has calendar</rdfs:label>
    <rdfs:isDefinedBy rdf:resource="http://e-editiones.ch/ontology/calendar#"/>
    <rdfs:domain rdf:resource="http://www.w3.org/2000/01/rdf-schema#Resource"/>
    <rdfs:label xml:lang="de">hat Kalender</rdfs:label>
  </owl:ObjectProperty>
  <owl:DatatypeProperty rdf:about="http://e-editiones.ch/ontology/calendar#hasJulianDate">
    <rdfs:isDefinedBy rdf:resource="http://e-editiones.ch/ontology/calendar#"/>
    <rdfs:domain rdf:resource="http://www.w3.org/2000/01/rdf-schema#Resource"/>
    <rdfs:range>
      <rdfs:Datatype rdf:about="http://e-editiones.ch/ontology/calendar#julianDate">
        <rdfs:label xml:lang="de">Datentyp julianisches Datum</rdfs:label>
        <rdfs:isDefinedBy rdf:resource="http://e-editiones.ch/ontology/calendar#"/>
        <rdfs:comment xml:lang="en">Datatype to type a date in the Julian calendar.</rdfs:comment>
        <rdfs:label xml:lang="en">Julian date datatype</rdfs:label>
      </rdfs:Datatype>
    </rdfs:range>
    <rdfs:label xml:lang="de">hat julianisches Datum</rdfs:label>
    <rdfs:label xml:lang="en">has Julian date</rdfs:label>
    <rdfs:comment xml:lang="en">Relating something to its Julian date.</rdfs:comment>
  </owl:DatatypeProperty>
  <owl:ObjectProperty rdf:about="http://e-editiones.ch/ontology/calendar#endYearLiteralToCenturyPeriod">
    <rdfs:label xml:lang="de">Endjahrliteral zu Jahrhundert</rdfs:label>
    <rdfs:domain rdf:resource="http://www.w3.org/1999/02/22-rdf-syntax-ns#List"/>
    <rdfs:comment xml:lang="en">Relating a list with a century end year literal and its calendar to the list with the calendar-dependent start and end date typed literal, and start and end Julian Day Number of the century.</rdfs:comment>
    <rdfs:range rdf:resource="http://www.w3.org/1999/02/22-rdf-syntax-ns#List"/>
    <skos:note xml:lang="en">Used in the premise of an N3-rule to invoke the backward N3-rule converting a century end year literal to the described object list, making explicit the start and end of the century for interval calculus in temporal reasoning.</skos:note>
    <rdfs:label xml:lang="en">end year literal to century period</rdfs:label>
    <skos:note xml:lang="en">Used in case of an accuracy of a century for an event time indicator, e.g. Gregorian death year '14..'.</skos:note>
    <rdfs:isDefinedBy rdf:resource="http://e-editiones.ch/ontology/calendar#"/>
  </owl:ObjectProperty>
  <owl:DatatypeProperty rdf:about="http://e-editiones.ch/ontology/calendar#hasStartJulianDayNumber">
    <rdfs:label xml:lang="en">has start Julian Day Number</rdfs:label>
    <rdfs:range>
      <rdfs:Datatype rdf:about="http://e-editiones.ch/ontology/calendar#julianDayNumber">
        <rdfs:label xml:lang="de">Datentyp julianische Tagesnummer</rdfs:label>
        <rdfs:comment xml:lang="en">Datatype to type a Julian Day Number integer.</rdfs:comment>
        <rdfs:comment xml:lang="en">The Julian Day Number (JDN) is the integer assigned to a whole solar day in the Julian day count starting from noon Universal time, with Julian Day Number 0 assigned to the day starting at noon on Monday, January 1, 4713 BC, proleptic Julian calendar (November 24, 4714 BC, in the proleptic Gregorian calendar), a date at which three multi-year cycles started (Indiction, Solar, and Lunar cycles) and which precedes any date in recorded human history.</rdfs:comment>
        <rdfs:label xml:lang="en">Julian Day Number datatype</rdfs:label>
        <rdfs:subClassOf rdf:resource="http://www.w3.org/2001/XMLSchema#integer"/>
        <rdfs:isDefinedBy rdf:resource="http://e-editiones.ch/ontology/calendar#"/>
      </rdfs:Datatype>
    </rdfs:range>
    <skos:note xml:lang="en">Used in an N3-rule to convert a calendar start date literal list of a year or year-month period to a start Julian Day Number integer.</skos:note>
    <rdfs:domain rdf:resource="http://e-editiones.ch/ontology/event#Event"/>
    <rdfs:comment xml:lang="en">Relating something to its start Julian Day Number.</rdfs:comment>
    <rdfs:label xml:lang="de">hat Start-julianische Tagesnummer</rdfs:label>
    <rdfs:subPropertyOf>
      <owl:DatatypeProperty rdf:about="http://e-editiones.ch/ontology/calendar#hasJulianDayNumber">
        <rdfs:label xml:lang="en">has Julian Day Number</rdfs:label>
        <rdfs:domain rdf:resource="http://www.w3.org/2000/01/rdf-schema#Resource"/>
        <skos:note xml:lang="en">Used in an N3-rule to convert a calendar date literal list to a Julian Day Number.</skos:note>
        <rdfs:comment xml:lang="en">Relating something to its Julian Day Number.</rdfs:comment>
        <rdfs:label xml:lang="de">hat julianische Tagesnummer</rdfs:label>
        <rdfs:range rdf:resource="http://e-editiones.ch/ontology/calendar#julianDayNumber"/>
        <rdfs:isDefinedBy rdf:resource="http://e-editiones.ch/ontology/calendar#"/>
      </owl:DatatypeProperty>
    </rdfs:subPropertyOf>
    <rdfs:isDefinedBy rdf:resource="http://e-editiones.ch/ontology/calendar#"/>
  </owl:DatatypeProperty>
  <owl:DatatypeProperty rdf:about="http://e-editiones.ch/ontology/calendar#prolepticJulianListToJulianDayNumber">
    <rdfs:label xml:lang="en">proleptic Julian list to Julian Day Number</rdfs:label>
    <rdfs:domain rdf:resource="http://www.w3.org/1999/02/22-rdf-syntax-ns#List"/>
    <rdfs:isDefinedBy rdf:resource="http://e-editiones.ch/ontology/calendar#"/>
    <rdfs:range rdf:resource="http://e-editiones.ch/ontology/calendar#julianDayNumber"/>
    <rdfs:comment xml:lang="en">Relating a proleptic Julian date as a list of literals to its Julian Day Number.</rdfs:comment>
    <rdfs:label xml:lang="de">proleptisch julianische Liste zu julianischer Tagesnummer</rdfs:label>
    <skos:note xml:lang="en">Used in the premise of the backward 'dateLiteralToDate', 'yearLiteralToPeriod', and 'yearMonthLiteralToPeriod' N3-rules to invoke its backward 'prolepticJulianListToJulianDayNumber' N3-rule converting a proleptic Julian date literal list to its Julian Day Number.</skos:note>
  </owl:DatatypeProperty>
  <owl:DatatypeProperty rdf:about="http://e-editiones.ch/ontology/calendar#hasJulianStartDate">
    <rdfs:domain rdf:resource="http://e-editiones.ch/ontology/event#Event"/>
    <rdfs:isDefinedBy rdf:resource="http://e-editiones.ch/ontology/calendar#"/>
    <rdfs:label xml:lang="en">has Julian start date</rdfs:label>
    <rdfs:label xml:lang="de">hat julianisches Startdatum</rdfs:label>
    <rdfs:range rdf:resource="http://e-editiones.ch/ontology/calendar#julianDate"/>
    <rdfs:comment xml:lang="en">Relating something to its Julian start date.</rdfs:comment>
  </owl:DatatypeProperty>
  <owl:DatatypeProperty rdf:about="http://e-editiones.ch/ontology/calendar#gregorianListToDate">
    <rdfs:domain rdf:resource="http://www.w3.org/1999/02/22-rdf-syntax-ns#List"/>
    <rdfs:range rdf:resource="http://www.w3.org/2001/XMLSchema#date"/>
    <rdfs:label xml:lang="en">Gregorian list to date</rdfs:label>
    <rdfs:comment xml:lang="en">Relating a Gregorian date as a list of literals to its date typed literal.</rdfs:comment>
    <skos:note xml:lang="en">Used in the premise of the backward 'dateLiteralToDate', 'yearLiteralToPeriod', and 'yearMonthLiteralToPeriod' N3-rules for the Gregorian calendar to invoke its backward 'gregorianListToDate' N3-rule converting a Gregorian date literal list to its date typed literal.</skos:note>
    <rdfs:isDefinedBy rdf:resource="http://e-editiones.ch/ontology/calendar#"/>
    <rdfs:label xml:lang="de">gregorianische Liste zu Datum</rdfs:label>
  </owl:DatatypeProperty>
  <owl:ObjectProperty rdf:about="http://e-editiones.ch/ontology/calendar#yearLiteralToDecadePeriod">
    <rdfs:comment xml:lang="en">Relating a list with a decade start year literal and its calendar to the list with the calendar-dependent start and end date typed literal, and start and end Julian Day Number of the decade.</rdfs:comment>
    <rdfs:domain rdf:resource="http://www.w3.org/1999/02/22-rdf-syntax-ns#List"/>
    <rdfs:isDefinedBy rdf:resource="http://e-editiones.ch/ontology/calendar#"/>
    <rdfs:range rdf:resource="http://www.w3.org/1999/02/22-rdf-syntax-ns#List"/>
    <skos:note xml:lang="en">Used in the premise of an N3-rule to invoke the backward N3-rule converting a decade start year literal to the described object list, making explicit the start and end of the decade for interval calculus in temporal reasoning.</skos:note>
    <rdfs:label xml:lang="de">Jahrliteral zu Jahrzehnt</rdfs:label>
    <rdfs:label xml:lang="en">year literal to decade period</rdfs:label>
  </owl:ObjectProperty>
  <owl:DatatypeProperty rdf:about="http://e-editiones.ch/ontology/calendar#hasGregorianStartDate">
    <rdfs:domain rdf:resource="http://e-editiones.ch/ontology/event#Event"/>
    <rdfs:isDefinedBy rdf:resource="http://e-editiones.ch/ontology/calendar#"/>
    <rdfs:comment xml:lang="en">Relating an event to its Gregorian start date.</rdfs:comment>
    <rdfs:label xml:lang="de">hat gregorianisches Startdatum</rdfs:label>
    <rdfs:label xml:lang="en">has Gregorian start date</rdfs:label>
    <rdfs:range rdf:resource="http://www.w3.org/2001/XMLSchema#date"/>
  </owl:DatatypeProperty>
  <owl:DatatypeProperty rdf:about="http://e-editiones.ch/ontology/calendar#hasJulianEndDate">
    <rdfs:comment xml:lang="en">Relating something to its Julian end date.</rdfs:comment>
    <rdfs:label xml:lang="de">hat julianisches Enddatum</rdfs:label>
    <rdfs:domain rdf:resource="http://e-editiones.ch/ontology/event#Event"/>
    <rdfs:range rdf:resource="http://e-editiones.ch/ontology/calendar#julianDate"/>
    <rdfs:label xml:lang="en">has Julian end date</rdfs:label>
    <rdfs:isDefinedBy rdf:resource="http://e-editiones.ch/ontology/calendar#"/>
  </owl:DatatypeProperty>
  <owl:DatatypeProperty rdf:about="http://e-editiones.ch/ontology/calendar#julianListToDate">
    <rdfs:label xml:lang="de">julianische Liste zu Datum</rdfs:label>
    <rdfs:isDefinedBy rdf:resource="http://e-editiones.ch/ontology/calendar#"/>
    <rdfs:range rdf:resource="http://e-editiones.ch/ontology/calendar#julianDate"/>
    <rdfs:domain rdf:resource="http://www.w3.org/1999/02/22-rdf-syntax-ns#List"/>
    <rdfs:label xml:lang="en">Julian list to date</rdfs:label>
    <rdfs:comment xml:lang="en">Relating a Julian date as a list of literals to its date typed literal.</rdfs:comment>
    <skos:note xml:lang="en">Used in the premise of the backward 'dateLiteralToDate' N3-rules for the Julian calendar to invoke its backward 'julianListToDate' N3-rule converting a Julian date literal list to its date typed literal.</skos:note>
  </owl:DatatypeProperty>
  <owl:DatatypeProperty rdf:about="http://e-editiones.ch/ontology/calendar#hasProlepticJulianEndDate">
    <rdfs:label xml:lang="de">hat proleptisch julianisches Enddatum</rdfs:label>
    <rdfs:isDefinedBy rdf:resource="http://e-editiones.ch/ontology/calendar#"/>
    <rdfs:label xml:lang="en">has proleptic Julian end date</rdfs:label>
    <rdfs:comment xml:lang="en">Relating something to its proleptic Julian end date.</rdfs:comment>
    <rdfs:range>
      <rdfs:Datatype rdf:about="http://e-editiones.ch/ontology/calendar#prolepticJulianDate">
        <rdfs:label xml:lang="en">proleptic Julian date datatype</rdfs:label>
        <rdfs:comment xml:lang="en">Datatype to type a date in the proleptic Julian calendar.</rdfs:comment>
        <rdfs:label xml:lang="de">Datentyp proleptisches julianisches Datum</rdfs:label>
        <rdfs:isDefinedBy rdf:resource="http://e-editiones.ch/ontology/calendar#"/>
      </rdfs:Datatype>
    </rdfs:range>
    <rdfs:domain rdf:resource="http://e-editiones.ch/ontology/event#Event"/>
  </owl:DatatypeProperty>
  <owl:DatatypeProperty rdf:about="http://e-editiones.ch/ontology/calendar#hasGregorianDate">
    <rdfs:isDefinedBy rdf:resource="http://e-editiones.ch/ontology/calendar#"/>
    <rdfs:comment xml:lang="en">Relating something to its Gregorian date.</rdfs:comment>
    <rdfs:label xml:lang="en">has Gregorian date</rdfs:label>
    <rdfs:label xml:lang="de">hat gregorianisches Datum</rdfs:label>
    <rdfs:domain rdf:resource="http://www.w3.org/2000/01/rdf-schema#Resource"/>
    <rdfs:range rdf:resource="http://www.w3.org/2001/XMLSchema#date"/>
  </owl:DatatypeProperty>
  <owl:DatatypeProperty rdf:about="http://e-editiones.ch/ontology/calendar#hasProlepticJulianDate">
    <rdfs:range rdf:resource="http://e-editiones.ch/ontology/calendar#prolepticJulianDate"/>
    <rdfs:label xml:lang="en">has proleptic Julian date</rdfs:label>
    <rdfs:isDefinedBy rdf:resource="http://e-editiones.ch/ontology/calendar#"/>
    <rdfs:comment xml:lang="en">Relating something to its proleptic Julian date.</rdfs:comment>
    <rdfs:domain rdf:resource="http://www.w3.org/2000/01/rdf-schema#Resource"/>
    <rdfs:label xml:lang="de">hat proleptisch julianisches Datum</rdfs:label>
  </owl:DatatypeProperty>
  <owl:DatatypeProperty rdf:about="http://e-editiones.ch/ontology/calendar#julianSetListToDate">
    <rdfs:domain rdf:resource="http://www.w3.org/1999/02/22-rdf-syntax-ns#List"/>
    <skos:note xml:lang="en">Used in the premise of the backward 'yearLiteralToPeriod' and 'yearMonthLiteralToPeriod' N3-rules for the Julian calendar to invoke its backward 'julianSetListToDate' N3-rule converting a Julian date literal list to its date typed literal.</skos:note>
    <rdfs:range rdf:resource="http://e-editiones.ch/ontology/calendar#julianDate"/>
    <rdfs:label xml:lang="en">Julian set date list to date</rdfs:label>
    <rdfs:isDefinedBy rdf:resource="http://e-editiones.ch/ontology/calendar#"/>
    <rdfs:label xml:lang="de">gesetzte julianische Datumliste zu Datum</rdfs:label>
    <rdfs:comment xml:lang="en">Relating a Julian date literal list with set month and day to its date typed literal.</rdfs:comment>
  </owl:DatatypeProperty>
  <owl:Ontology rdf:about="http://e-editiones.ch/ontology/calendar">
    <owl:versionInfo rdf:datatype="http://www.w3.org/2001/XMLSchema#date">2020-06-11</owl:versionInfo>
    <dct:contributor xml:lang="en">Rebekka Pl√ºss, research assistant and software developer, University of Basel, Switzerland</dct:contributor>
    <dct:publisher xml:lang="en">Universities of Basel, Bern, and Z√ºrich, Switzerland</dct:publisher>
    <dct:license rdf:resource="http://creativecommons.org/licenses/by/3.0/"/>
    <dct:description xml:lang="en">Formal description of calendar, subclasses, related classes, and properties.</dct:description>
    <dct:title xml:lang="en">calendar-ontology</dct:title>
    <dct:creator xml:lang="en">Hans Cools, MD, knowledge engineer, ontologist, software developer, University of Basel, Switzerland</dct:creator>
    <dct:issued rdf:datatype="http://www.w3.org/2001/XMLSchema#dateTime">2019-12-28T13:45:00+01:00</dct:issued>
  </owl:Ontology>
  <owl:DatatypeProperty rdf:about="http://e-editiones.ch/ontology/calendar#prolepticJulianListToDate">
    <rdfs:domain rdf:resource="http://www.w3.org/1999/02/22-rdf-syntax-ns#List"/>
    <skos:note xml:lang="en">Used in the premise of the backward 'dateLiteralToDate' N3-rules for the proleptic Julian calendar to invoke its backward 'prolepticJulianListToDate' N3-rule converting a proleptic Julian date literal list to its date typed literal.</skos:note>
    <rdfs:label xml:lang="en">proleptic Julian list to date</rdfs:label>
    <rdfs:label xml:lang="de">proleptisch julianische Liste zu Datum</rdfs:label>
    <rdfs:range rdf:resource="http://e-editiones.ch/ontology/calendar#prolepticJulianDate"/>
    <rdfs:comment xml:lang="en">Relating a proleptic Julian date as a list of literals to its date typed literal.</rdfs:comment>
    <rdfs:isDefinedBy rdf:resource="http://e-editiones.ch/ontology/calendar#"/>
  </owl:DatatypeProperty>
  <owl:DatatypeProperty rdf:about="http://e-editiones.ch/ontology/calendar#julianDayNumeralToGregorianDate">
    <skos:note xml:lang="en">Used in the premise of an N3-rule to invoke the eponymous backward N3-rule to convert a Julian Day Numeral, i.e. not typed with calendar:julianDayNumber, to its Gregorian date typed literal.</skos:note>
    <rdfs:range rdf:resource="http://www.w3.org/2001/XMLSchema#date"/>
    <rdfs:comment xml:lang="en">Relating a Julian Day Numeral to its Gregorian date typed literal.</rdfs:comment>
    <rdfs:label xml:lang="de">julianischer Tag-Numeral zu gregorianischem Datum</rdfs:label>
    <rdfs:isDefinedBy rdf:resource="http://e-editiones.ch/ontology/calendar#"/>
    <rdfs:label xml:lang="en">Julian Day Numeral to Gregorian date</rdfs:label>
    <rdfs:domain rdf:resource="http://www.w3.org/2001/XMLSchema#nonNegativeInteger"/>
  </owl:DatatypeProperty>
  <calendar:Calendar rdf:about="http://e-editiones.ch/ontology/calendar#prolepticJulianCalendar">
    <rdfs:label xml:lang="it">calendario juliano proleptico</rdfs:label>
    <rdfs:label xml:lang="de">proleptischer julianischer Kalender</rdfs:label>
    <rdfs:comment xml:lang="en">Produced by extending the Julian calendar backward to dates preceding its use in stable form from 4 AD on.</rdfs:comment>
    <rdfs:label xml:lang="fr">calendrier julien proleptique</rdfs:label>
    <rdfs:isDefinedBy rdf:resource="http://e-editiones.ch/ontology/calendar#"/>
    <rdfs:label xml:lang="en">proleptic Julian calendar</rdfs:label>
    <skos:note xml:lang="en">There is no proleptic Julian year 0. Year 1 BC is followed by year 1 AD.</skos:note>
  </calendar:Calendar>
  <owl:DatatypeProperty rdf:about="http://e-editiones.ch/ontology/calendar#hasEndJulianDayNumber">
    <rdfs:label xml:lang="de">hat End-julianische Tagesnummer</rdfs:label>
    <rdfs:label xml:lang="en">has end Julian Day Number</rdfs:label>
    <rdfs:subPropertyOf rdf:resource="http://e-editiones.ch/ontology/calendar#hasJulianDayNumber"/>
    <skos:note xml:lang="en">Used in an N3-rule to convert a calendar end date literal list of a year or year-month period to an end Julian Day Number integer.</skos:note>
    <rdfs:domain rdf:resource="http://e-editiones.ch/ontology/event#Event"/>
    <rdfs:comment xml:lang="en">Relating an event to its end Julian Day Number.</rdfs:comment>
    <rdfs:isDefinedBy rdf:resource="http://e-editiones.ch/ontology/calendar#"/>
    <rdfs:range rdf:resource="http://e-editiones.ch/ontology/calendar#julianDayNumber"/>
  </owl:DatatypeProperty>
  <owl:DatatypeProperty rdf:about="http://e-editiones.ch/ontology/calendar#hasProlepticJulianStartDate">
    <rdfs:label xml:lang="en">has proleptic Julian start date</rdfs:label>
    <rdfs:isDefinedBy rdf:resource="http://e-editiones.ch/ontology/calendar#"/>
    <rdfs:comment xml:lang="en">Relating something to its proleptic Julian start date.</rdfs:comment>
    <rdfs:label xml:lang="de">hat proleptisch julianisches Startdatum</rdfs:label>
    <rdfs:range rdf:resource="http://e-editiones.ch/ontology/calendar#prolepticJulianDate"/>
    <rdfs:domain rdf:resource="http://e-editiones.ch/ontology/event#Event"/>
  </owl:DatatypeProperty>
  <owl:DatatypeProperty rdf:about="http://e-editiones.ch/ontology/calendar#gregorianListToJulianDayNumber">
    <rdfs:label xml:lang="en">Gregorian list to Julian Day Number</rdfs:label>
    <rdfs:domain rdf:resource="http://www.w3.org/1999/02/22-rdf-syntax-ns#List"/>
    <rdfs:isDefinedBy rdf:resource="http://e-editiones.ch/ontology/calendar#"/>
    <skos:note xml:lang="en">Used in the premise of the backward 'dateLiteralToDate', 'yearLiteralToPeriod', and 'yearMonthLiteralToPeriod' N3-rules for the Gregorian calendar to invoke its backward 'gregorianListToJulianDayNumber' N3-rule converting a Gregorian date literal list to its Julian Day Number.</skos:note>
    <rdfs:label xml:lang="de">gregorianische Liste zu julianische Tagesnummer</rdfs:label>
    <rdfs:range rdf:resource="http://e-editiones.ch/ontology/calendar#julianDayNumber"/>
    <rdfs:comment xml:lang="en">Relating a Gregorian date as a list of literals to its Julian Day Number.</rdfs:comment>
  </owl:DatatypeProperty>
  <owl:ObjectProperty rdf:about="http://e-editiones.ch/ontology/calendar#startYearLiteralToCenturyPeriod">
    <rdfs:label xml:lang="en">start year literal to century period</rdfs:label>
    <skos:note xml:lang="en">Used in case of an accuracy of a century for an event time indicator, e.g. Gregorian death year '14..'.</skos:note>
    <rdfs:isDefinedBy rdf:resource="http://e-editiones.ch/ontology/calendar#"/>
    <skos:note xml:lang="en">Used in the premise of an N3-rule to invoke the backward N3-rule converting a century start year literal to the described object list, making explicit the start and end of the century for interval calculus in temporal reasoning.</skos:note>
    <rdfs:domain rdf:resource="http://www.w3.org/1999/02/22-rdf-syntax-ns#List"/>
    <rdfs:label xml:lang="de">Startjahrliteral zu Jahrhundert</rdfs:label>
    <rdfs:range rdf:resource="http://www.w3.org/1999/02/22-rdf-syntax-ns#List"/>
    <rdfs:comment xml:lang="en">Relating a list with a century start year literal and its calendar to the list with the calendar-dependent start and end date typed literal, and start and end Julian Day Number of the century.</rdfs:comment>
  </owl:ObjectProperty>
  <calendar:Calendar rdf:about="http://e-editiones.ch/ontology/calendar#gregorianCalendar">
    <rdfs:label xml:lang="fr">calendrier gr√©gorien</rdfs:label>
    <rdfs:label xml:lang="it">calendario gregoriano</rdfs:label>
    <rdfs:comment xml:lang="en">Calendar introduced on 15 October 1582 AD by Pope Gregory XIII, and a correction of the Julian calendar. It is based on a solar year of 365 days. Every fourth year is a leap year of 366 days except for centenary years not evenly divisible by 400.</rdfs:comment>
    <rdfs:isDefinedBy rdf:resource="http://e-editiones.ch/ontology/calendar#"/>
    <skos:note xml:lang="en">Has 365.2425 days or 365 days, 5 hours, 49 minutes and 12 seconds per year. This number is used in temoral reasoning.</skos:note>
    <rdfs:label xml:lang="de">gregorianischer Kalender</rdfs:label>
    <rdfs:label xml:lang="en">Gregorian calendar</rdfs:label>
  </calendar:Calendar>
  <owl:DatatypeProperty rdf:about="http://e-editiones.ch/ontology/calendar#prolepticJulianSetListToDate">
    <rdfs:comment xml:lang="en">Relating a proleptic Julian date literal list with set month and day, to its date typed literal.</rdfs:comment>
    <rdfs:domain rdf:resource="http://www.w3.org/1999/02/22-rdf-syntax-ns#List"/>
    <rdfs:range rdf:resource="http://e-editiones.ch/ontology/calendar#prolepticJulianDate"/>
    <rdfs:isDefinedBy rdf:resource="http://e-editiones.ch/ontology/calendar#"/>
    <rdfs:label xml:lang="en">proleptic Julian set date list to date</rdfs:label>
    <skos:note xml:lang="en">Used in the premise of the backward 'yearLiteralToPeriod' and 'yearMonthLiteralToPeriod' N3-rules for the proleptic Julian calendar to invoke its backward 'prolepticJulianSetListToDate' N3-rule converting a proleptic Julian date literal list to its date typed literal.</skos:note>
    <rdfs:label xml:lang="de">gesetzte proleptisch julianische Datumliste zu Datum</rdfs:label>
  </owl:DatatypeProperty>
  <owl:ObjectProperty rdf:about="http://e-editiones.ch/ontology/calendar#yearLiteralToPeriod">
    <rdfs:label xml:lang="en">year literal to period</rdfs:label>
    <rdfs:comment xml:lang="en">Relating a calendar year literal to the list with the calendar-dependent start and end date typed literal, and start and end Julian Day Number of the year.</rdfs:comment>
    <rdfs:range rdf:resource="http://www.w3.org/1999/02/22-rdf-syntax-ns#List"/>
    <rdfs:domain rdf:resource="http://www.w3.org/1999/02/22-rdf-syntax-ns#List"/>
    <skos:note xml:lang="en">Used in the premise of an N3-rule to invoke the backward N3-rule converting a year literal to the described list, making explicit the start and end of the year for interval calculus in temporal reasoning.</skos:note>
    <rdfs:label xml:lang="de">Jahrliteral zu Zeitraum</rdfs:label>
    <rdfs:isDefinedBy rdf:resource="http://e-editiones.ch/ontology/calendar#"/>
  </owl:ObjectProperty>
  <calendar:Calendar rdf:about="http://e-editiones.ch/ontology/calendar#julianCalendar">
    <rdfs:label xml:lang="it">calendario juliano</rdfs:label>
    <rdfs:label xml:lang="de">julianischer Kalender</rdfs:label>
    <rdfs:isDefinedBy rdf:resource="http://e-editiones.ch/ontology/calendar#"/>
    <rdfs:label xml:lang="fr">calendrier julien</rdfs:label>
    <skos:note xml:lang="en">Has 365.25 days/year. This number is used in temoral reasoning.</skos:note>
    <rdfs:comment xml:lang="en">Calendar introduced in 46 BC in Rome by Julius Caesar. It is based on a solar year of 365 days. There are 12 months of 30 or 31 days, except for February, which has 28 days with the exception of every leap year when it has 29 days. Every fourth year and centenary year is a leap year of 366 days. The beginning of a year is not fixed on January 1. It was replaced by the Gregorian calendar in 1582 AD.</rdfs:comment>
    <skos:note xml:lang="en">A year that is exactly divisible by four is a leap year, except for years that are exactly divisible by 100, but these centurial years are leap years if they are exactly divisible by 400. For example, the years 1700, 1800, and 1900 are not leap years, but the year 2000 is.</skos:note>
    <rdfs:label xml:lang="en">Julian calendar</rdfs:label>
  </calendar:Calendar>
  <owl:DatatypeProperty rdf:about="http://e-editiones.ch/ontology/calendar#checkGregorianLeapYear">
    <rdfs:label xml:lang="de">gregorianisches Schaltjahr pr√ºfen</rdfs:label>
    <rdfs:domain rdf:resource="http://www.w3.org/1999/02/22-rdf-syntax-ns#List"/>
    <rdfs:label xml:lang="en">check Gregorian leap year</rdfs:label>
    <rdfs:isDefinedBy rdf:resource="http://e-editiones.ch/ontology/calendar#"/>
    <rdfs:comment xml:lang="en">Relating a Gregorian date as a list of literals to the message about the year being leap or not.</rdfs:comment>
    <skos:note xml:lang="en">Used in the premise of the backward 'dateLiteralToDate', 'yearLiteralToPeriod', and 'yearMonthLiteralToPeriod' N3-rules for the Gregorian calendar to invoke its backward 'checkGregorianLeapYear' N3-rules returning the literal message for the year being leap or not.</skos:note>
    <rdfs:range rdf:resource="http://www.w3.org/2000/01/rdf-schema#Literal"/>
  </owl:DatatypeProperty>
  <owl:ObjectProperty rdf:about="http://e-editiones.ch/ontology/calendar#yearMonthLiteralToPeriod">
    <rdfs:label xml:lang="en">year month literal to period</rdfs:label>
    <rdfs:domain rdf:resource="http://www.w3.org/1999/02/22-rdf-syntax-ns#List"/>
    <skos:note xml:lang="en">Used in the premise of an N3-rule to invoke the backward N3-rule converting a year-month literal list to the described object list, making explicit the start and end of the month for interval calculus in temporal reasoning.</skos:note>
    <rdfs:range rdf:resource="http://www.w3.org/1999/02/22-rdf-syntax-ns#List"/>
    <rdfs:comment xml:lang="en">Relating a calendar year-month literal list to the list with the calendar-dependent start and end date typed literal, and start and end Julian Day Number of the month.</rdfs:comment>
    <rdfs:label xml:lang="de">Jahr- und Monatliteral zu Zeitraum</rdfs:label>
    <rdfs:isDefinedBy rdf:resource="http://e-editiones.ch/ontology/calendar#"/>
  </owl:ObjectProperty>
  <owl:DatatypeProperty rdf:about="http://e-editiones.ch/ontology/calendar#hasMessageLiteral">
    <skos:note xml:lang="en">Used in an N3-rule; e.g. checking on leap year: "Has leap year."; e.g. checking consistency of e.g. month number, in case &gt; 12: "There are only 12 months in the Gregorian, Julian or proleptic Julian calendar." </skos:note>
    <rdfs:range rdf:resource="http://www.w3.org/2000/01/rdf-schema#Literal"/>
    <rdfs:isDefinedBy rdf:resource="http://e-editiones.ch/ontology/calendar#"/>
    <rdfs:label xml:lang="de">hat Nachrichtliteral</rdfs:label>
    <rdfs:label xml:lang="en">has message literal</rdfs:label>
    <rdfs:comment xml:lang="en">Relating something to a message literal about a calendar related time expression about that something.</rdfs:comment>
    <rdfs:domain rdf:resource="http://www.w3.org/2000/01/rdf-schema#Resource"/>
  </owl:DatatypeProperty>
  <owl:DatatypeProperty rdf:about="http://e-editiones.ch/ontology/calendar#hasGregorianEndDate">
    <rdfs:range rdf:resource="http://www.w3.org/2001/XMLSchema#date"/>
    <rdfs:domain rdf:resource="http://e-editiones.ch/ontology/event#Event"/>
    <rdfs:comment xml:lang="en">Relating an event to its Gregorian end date.</rdfs:comment>
    <rdfs:label xml:lang="de">hat gregorianisches Enddatum</rdfs:label>
    <rdfs:label xml:lang="en">has Gregorian end date</rdfs:label>
    <rdfs:isDefinedBy rdf:resource="http://e-editiones.ch/ontology/calendar#"/>
  </owl:DatatypeProperty>
  <owl:DatatypeProperty rdf:about="http://e-editiones.ch/ontology/calendar#julianListToJulianDayNumber">
    <rdfs:comment xml:lang="en">Relating a Julian date as a list of literals to its Julian Day Number.</rdfs:comment>
    <rdfs:domain rdf:resource="http://www.w3.org/1999/02/22-rdf-syntax-ns#List"/>
    <rdfs:range rdf:resource="http://e-editiones.ch/ontology/calendar#julianDayNumber"/>
    <rdfs:isDefinedBy rdf:resource="http://e-editiones.ch/ontology/calendar#"/>
    <rdfs:label xml:lang="de">julianische Liste zu julianische Tagesnummer</rdfs:label>
    <skos:note xml:lang="en">Used in the premise of the backward 'dateLiteralToDate', 'yearLiteralToPeriod', and 'yearMonthLiteralToPeriod' N3-rules to invoke its backward 'julianListToJulianDayNumber' N3-rule converting a Julian date literal list to its Julian Day Number.</skos:note>
    <rdfs:label xml:lang="en">Julian list to Julian Day Number</rdfs:label>
  </owl:DatatypeProperty>
  <rdfs:Class rdf:about="http://e-editiones.ch/ontology/calendar#Calendar">
    <rdfs:label xml:lang="en">calendar</rdfs:label>
    <rdfs:subClassOf rdf:resource="http://e-editiones.ch/ontology/concept#Information"/>
    <rdfs:label xml:lang="de">Kalender</rdfs:label>
    <rdfs:label xml:lang="it">calendario</rdfs:label>
    <rdfs:comment xml:lang="en">System of reckoning time in which the beginning, length, and divisions of a year are defined, sometimes along with multiyear cycles.</rdfs:comment>
    <rdfs:isDefinedBy rdf:resource="http://e-editiones.ch/ontology/calendar#"/>
    <rdfs:label xml:lang="fr">calendrier</rdfs:label>
  </rdfs:Class>
</rdf:RDF>
